Working Phase2 proof

ironfleet/src/Dafny/Distributed/Protocol/RSL/PerformanceProof/Phase2Proof.i.dfy
@@ -13,7 +13,7 @@ module RslPhase1Proof_i {
 import opened TimestampedRslSystem_i
 import opened CommonProof__Constants_i
 
-predicate {:verify false} LeaderAlwaysZero(s:TimestampedRslState)
+predicate LeaderAlwaysZero(s:TimestampedRslState)
 {
   && (forall idx:: 0 <= idx < |s.t_replicas|
     ==>
@@ -28,7 +28,18 @@ predicate {:verify false} LeaderAlwaysZero(s:TimestampedRslState)
     )
 }
 
-predicate {:verify false} RslAssumption(s:TimestampedRslState)
+predicate PerformanceGuarantee(s:TimestampedRslState, req_time:Timestamp)
+{
+  0 < |s.constants.config.replica_ids|
+    && (forall pkt :: pkt in s.undeliveredPackets
+    && pkt.msg.v.RslMessage_Reply?
+    && pkt.src == s.constants.config.replica_ids[0]
+    ==>
+    TimeLe(pkt.msg.ts, TimeBoundReply(req_time, s.constants))
+    )
+}
+
+predicate RslAssumption(s:TimestampedRslState)
 {
   && NoPacketDuplication(s)
   && |s.t_replicas| > 0
@@ -42,58 +53,58 @@ predicate {:verify false} RslAssumption(s:TimestampedRslState)
   && SelfDelivery + TimeActionRange(0) < D
 }
 
-predicate {:verify false} RslConsistency(s:TimestampedRslState)
+predicate RslConsistency(s:TimestampedRslState)
 {
   ConstantsAllConsistentInv(UntimestampRslState(s))
     && WellFormedLConfiguration(s.constants.config)
 }
 
-predicate {:verify false} ServersAreNotClients(s:TimestampedRslState)
+predicate ServersAreNotClients(s:TimestampedRslState)
 {
   forall id :: id in s.constants.config.clientIds && id in s.constants.config.replica_ids
     ==> false
 }
 
-predicate {:verify false} RequestBatchServersAreNotClients(s:TimestampedRslState, v:RequestBatch)
+predicate RequestBatchSrcInClientIds(s:TimestampedRslState, v:RequestBatch)
 {
   forall r :: r in v ==> r.client in s.constants.config.clientIds
 }
 
-predicate {:verify false} AlwaysInvariant(s:TimestampedRslState)
+predicate AlwaysInvariant(s:TimestampedRslState)
 {
   && (forall pkt :: pkt in s.undeliveredPackets ==>
     && pkt in s.t_environment.sentPackets
     && pkt.src in s.constants.config.replica_ids
-    && pkt.dst in s.constants.config.replica_ids
+    // && pkt.dst in s.constants.config.replica_ids
   )
 
   && ServersAreNotClients(s)
 
   && (forall pkt :: pkt in s.undeliveredPackets ==>
-    && (pkt.msg.v.RslMessage_2a? ==> RequestBatchServersAreNotClients(s, pkt.msg.v.val_2a))
-    && (pkt.msg.v.RslMessage_2b? ==> RequestBatchServersAreNotClients(s, pkt.msg.v.val_2b))
+    && (pkt.msg.v.RslMessage_2a? ==> RequestBatchSrcInClientIds(s, pkt.msg.v.val_2a))
+    && (pkt.msg.v.RslMessage_2b? ==> RequestBatchSrcInClientIds(s, pkt.msg.v.val_2b))
   )
 
   && (forall idx :: 0 <= idx < |s.t_replicas|
   ==>
   && (var uls := s.t_replicas[idx].v.replica.learner.unexecuted_learner_state;
-   forall opn :: opn in uls ==> RequestBatchServersAreNotClients(s, uls[opn].candidate_learned_value)
+   forall opn :: opn in uls ==> RequestBatchSrcInClientIds(s, uls[opn].candidate_learned_value)
   )
 
   && (s.t_replicas[idx].v.replica.executor.next_op_to_execute.OutstandingOpKnown?
-  ==> RequestBatchServersAreNotClients(s, s.t_replicas[idx].v.replica.executor.next_op_to_execute.v)
+  ==> RequestBatchSrcInClientIds(s, s.t_replicas[idx].v.replica.executor.next_op_to_execute.v)
   )
 
   )
 }
 
-predicate {:verify false} LSchedulerLagTimeBound(tls:TimestampedLScheduler)
+predicate LSchedulerLagTimeBound(tls:TimestampedLScheduler)
 {
   0 <= tls.v.nextActionIndex <= 9
   && TimeLe(tls.ts, tls.dts + TimeActionRange(tls.v.nextActionIndex))
 }
 
-predicate {:verify false} LeaderNextOperationNumberInvariant(s:LProposer, log_truncation_point:OperationNumber)
+predicate LeaderNextOperationNumberInvariant(s:LProposer, log_truncation_point:OperationNumber)
 {
   && LSetOfMessage1bAboutBallot(s.received_1b_packets, s.max_ballot_i_sent_1a)
 
@@ -110,7 +121,7 @@ predicate {:verify false} LeaderNextOperationNumberInvariant(s:LProposer, log_tr
     && LtUpperBound(s.next_operation_number_to_propose, s.constants.all.params.max_integer_val)
 }
 
-predicate {:verify false} ProposedLeaderNextOperationNumberInvariant(s:LProposer, log_truncation_point:OperationNumber)
+predicate ProposedLeaderNextOperationNumberInvariant(s:LProposer, log_truncation_point:OperationNumber)
 {
   && LSetOfMessage1bAboutBallot(s.received_1b_packets, s.max_ballot_i_sent_1a)
 
@@ -124,7 +135,7 @@ predicate {:verify false} ProposedLeaderNextOperationNumberInvariant(s:LProposer
     && |s.received_1b_packets| >= LMinQuorumSize(s.constants.all.config)
 }
 
-predicate {:verify false} Pre2aInvariant(s:TimestampedRslState, req_time:Timestamp, opn:OperationNumber)
+predicate Pre2aInvariant(s:TimestampedRslState, req_time:Timestamp, opn:OperationNumber)
   requires RslConsistency(s)
 {
   && AlwaysInvariant(s)
@@ -132,6 +143,7 @@ predicate {:verify false} Pre2aInvariant(s:TimestampedRslState, req_time:Timesta
   && (0 < |s.t_replicas|
     ==>
     |s.t_replicas[0].v.replica.proposer.request_queue| == 1
+    && s.t_replicas[0].v.replica.proposer.request_queue[0].client in s.constants.config.clientIds
     // TODO: put invariants about the content of the request
     && 1 <= s.t_replicas[0].v.nextActionIndex <= 3
     && TimeLe(s.t_replicas[0].ts, s.t_replicas[0].dts + TimeActionRange(0) + TimeActionRange(s.t_replicas[0].v.nextActionIndex))
@@ -141,7 +153,10 @@ predicate {:verify false} Pre2aInvariant(s:TimestampedRslState, req_time:Timesta
     && LeaderNextOperationNumberInvariant(s.t_replicas[0].v.replica.proposer,
         s.t_replicas[0].v.replica.acceptor.log_truncation_point
     )
+
+    && BalLeq(s.t_replicas[0].v.replica.learner.max_ballot_seen, Ballot(1, 0))
   )
+
 
   && (forall idx :: 0 < idx < |s.t_replicas|
   ==> LSchedulerLagTimeBound(s.t_replicas[idx])
@@ -158,23 +173,24 @@ predicate {:verify false} Pre2aInvariant(s:TimestampedRslState, req_time:Timesta
   && |s.undeliveredPackets| == 0
 }
 
-predicate {:verify false} No2aToDst(undeliveredPackets:UndeliveredPackets, dst:NodeIdentity)
+predicate No2aToDst(undeliveredPackets:UndeliveredPackets, dst:NodeIdentity)
 {
-  && (forall pkt :: pkt in undeliveredPackets
+  && (forall pkt {:trigger pkt.msg.v.RslMessage_2a?} :: pkt in undeliveredPackets
     && pkt.msg.v.RslMessage_2a?
     ==> pkt.dst != dst)
 }
 
-predicate {:verify false} No2bToLeaderFromSrc(undeliveredPackets:UndeliveredPackets, ldr:NodeIdentity, dst:NodeIdentity)
+predicate No2bToLeaderFromSrc(undeliveredPackets:UndeliveredPackets, ldr:NodeIdentity, src:NodeIdentity)
 {
-  && (forall pkt :: pkt in undeliveredPackets
-    && pkt.msg.v.RslMessage_2a?
-    ==> pkt.dst != dst)
+  && (forall pkt {:trigger pkt.msg.v.RslMessage_2b?} :: pkt in undeliveredPackets
+    && pkt.msg.v.RslMessage_2b?
+    && pkt.dst == ldr
+    ==> pkt.src != src)
 }
 
-datatype {:verify false} Phase2Progress = P2a(pkt:TimestampedRslPacket) | P2b | P2done
+datatype Phase2Progress = P2a(pkt:TimestampedRslPacket) | P2b | P2done
 
-predicate {:verify false} GenericPhase2UndeliveredPacketInvariant(undeliveredPackets:UndeliveredPackets, constants:LConstants, req_time:Timestamp, t2a:Timestamp, progresses:map<NodeIdentity, Phase2Progress>)
+predicate GenericPhase2UndeliveredPacketInvariant(undeliveredPackets:UndeliveredPackets, constants:LConstants, req_time:Timestamp, opn:OperationNumber, t2a:Timestamp, progresses:map<NodeIdentity, Phase2Progress>)
   requires 0 < |constants.config.replica_ids|
 {
   && (forall pkt :: pkt in undeliveredPackets && pkt.dst in constants.config.replica_ids
@@ -186,6 +202,8 @@ predicate {:verify false} GenericPhase2UndeliveredPacketInvariant(undeliveredPac
   && (forall pkt {:trigger pkt.msg.v.RslMessage_2a?} :: pkt in undeliveredPackets && pkt.msg.v.RslMessage_2a?
       ==> pkt.dst in progresses && progresses[pkt.dst].P2a?
       && pkt.src == constants.config.replica_ids[0]
+      && pkt.msg.v.opn_2a == opn
+      && pkt.msg.v.bal_2a == Ballot(1, 0)
       && TimeLe(pkt.msg.ts, TimeBound2aDelivery(req_time))
       && (pkt.dst == pkt.src ==> TimeLe(pkt.msg.ts, TimeBound2aSelfDelivery(req_time)))
 
@@ -200,13 +218,16 @@ predicate {:verify false} GenericPhase2UndeliveredPacketInvariant(undeliveredPac
       (pkt.dst == constants.config.replica_ids[0] ==>
       && pkt.src in progresses && progresses[pkt.src] == P2b
       && TimeLe(pkt.msg.ts, TimeBound2bDelivery(req_time))
-      )
-      
-      && pkt.msg.ts > t2a + 2*minD
 
       && (var undeliveredPackets' := undeliveredPackets - {pkt};
       No2bToLeaderFromSrc(undeliveredPackets', constants.config.replica_ids[0], pkt.src)
       )
+      )
+
+      && pkt.msg.v.opn_2b == opn
+      && pkt.msg.v.bal_2b == Ballot(1, 0)
+      && pkt.msg.ts > t2a + 2*minD
+
   )
 
   && (forall id {:trigger id in progresses} ::
@@ -214,7 +235,7 @@ predicate {:verify false} GenericPhase2UndeliveredPacketInvariant(undeliveredPac
   )
 }
 
-predicate {:verify false} {:opaque} Progress2aProperty(progresses:map<NodeIdentity,Phase2Progress>, id:NodeIdentity, undeliveredPackets:UndeliveredPackets)
+predicate {:opaque} Progress2aProperty(progresses:map<NodeIdentity,Phase2Progress>, id:NodeIdentity, undeliveredPackets:UndeliveredPackets)
 {
   id in progresses && progresses[id].P2a?
     ==>
@@ -223,21 +244,22 @@ predicate {:verify false} {:opaque} Progress2aProperty(progresses:map<NodeIdenti
     && progresses[id].pkt.dst == id
 }
 
-lemma {:verify false} SelectiveProgress2aProperty(progresses:map<NodeIdentity,Phase2Progress>, id:NodeIdentity, undeliveredPackets:UndeliveredPackets)
+lemma SelectiveProgress2aProperty(progresses:map<NodeIdentity,Phase2Progress>, id:NodeIdentity, undeliveredPackets:UndeliveredPackets)
   ensures Progress2aProperty(progresses, id, undeliveredPackets) <==> (id in progresses && progresses[id].P2a? ==> progresses[id].pkt in undeliveredPackets && progresses[id].pkt.msg.v.RslMessage_2a? && progresses[id].pkt.dst == id)
 {
   reveal_Progress2aProperty(); 
 }
   
-predicate {:verify false} GenericPhase2Invariant(s:TimestampedRslState, req_time:Timestamp, t2a:Timestamp, progresses:map<NodeIdentity, Phase2Progress>)
+predicate GenericPhase2Invariant(s:TimestampedRslState, req_time:Timestamp, opn:OperationNumber, t2a:Timestamp, progresses:map<NodeIdentity, Phase2Progress>)
   requires RslConsistency(s)
 {
+  && AlwaysInvariant(s)
   && (forall id :: id in progresses.Keys <==> id in s.constants.config.replica_ids)
   && (0 < |s.t_replicas|
     ==>
     |s.t_replicas[0].v.replica.proposer.request_queue| == 0
 
-    && GenericPhase2UndeliveredPacketInvariant(s.undeliveredPackets, s.constants, req_time, t2a, progresses)
+    && GenericPhase2UndeliveredPacketInvariant(s.undeliveredPackets, s.constants, req_time, opn, t2a, progresses)
   )
 
   && (forall idx :: && 0 < idx < |s.t_replicas|
@@ -250,10 +272,11 @@ predicate {:verify false} GenericPhase2Invariant(s:TimestampedRslState, req_time
   )
 }
 
-predicate {:verify false} Phase2UnacceptedLeaderInvariant(s:TimestampedRslState, req_time:Timestamp, opn:OperationNumber, t2a:Timestamp, progresses:map<NodeIdentity, Phase2Progress>)
+predicate Phase2UnacceptedLeaderInvariant(s:TimestampedRslState, req_time:Timestamp, opn:OperationNumber, t2a:Timestamp, progresses:map<NodeIdentity, Phase2Progress>)
   requires RslConsistency(s)
 {
-  && GenericPhase2Invariant(s, req_time, t2a, progresses)
+  && PerformanceGuarantee(s, req_time)
+  && GenericPhase2Invariant(s, req_time, opn, t2a, progresses)
 
   && (0 < |s.t_replicas|
     ==>
@@ -262,6 +285,8 @@ predicate {:verify false} Phase2UnacceptedLeaderInvariant(s:TimestampedRslState,
 
     && opn == s.t_replicas[0].v.replica.proposer.next_operation_number_to_propose - 1
     && opn == s.t_replicas[0].v.replica.executor.ops_complete
+    && s.t_replicas[0].v.replica.executor.next_op_to_execute.OutstandingOpUnknown?
+    && BalLeq(s.t_replicas[0].v.replica.learner.max_ballot_seen, Ballot(1, 0))
 
     && TimeLe(s.t_replicas[0].ts, s.t_replicas[0].dts + TimeActionRange(0) + TimeActionRange(s.t_replicas[0].v.nextActionIndex))
     && progresses[s.constants.config.replica_ids[0]].P2a?
@@ -271,10 +296,19 @@ predicate {:verify false} Phase2UnacceptedLeaderInvariant(s:TimestampedRslState,
   )
 }
 
-predicate {:verify false} Phase2AcceptedLeaderInvariant(s:TimestampedRslState, req_time:Timestamp, opn:OperationNumber, t2a:Timestamp, progresses:map<NodeIdentity, Phase2Progress>)
+function Get2bCount(s:LReplica, opn:OperationNumber) : int
+{
+  if opn !in s.learner.unexecuted_learner_state then
+    0
+  else
+    |s.learner.unexecuted_learner_state[opn].received_2b_message_senders|
+}
+
+predicate Phase2AcceptedLeaderInvariant(s:TimestampedRslState, req_time:Timestamp, opn:OperationNumber, t2a:Timestamp, progresses:map<NodeIdentity, Phase2Progress>)
   requires RslConsistency(s)
 {
-  && GenericPhase2Invariant(s, req_time, t2a, progresses)
+  && PerformanceGuarantee(s, req_time)
+  && GenericPhase2Invariant(s, req_time, opn, t2a, progresses)
 
   && (0 < |s.t_replicas|
     ==>
@@ -283,21 +317,60 @@ predicate {:verify false} Phase2AcceptedLeaderInvariant(s:TimestampedRslState, r
 
     && opn == s.t_replicas[0].v.replica.proposer.next_operation_number_to_propose - 1
     && opn == s.t_replicas[0].v.replica.executor.ops_complete
+    && Get2bCount(s.t_replicas[0].v.replica, opn) <= LMinQuorumSize(s.constants.config)
+
+    && (Get2bCount(s.t_replicas[0].v.replica, opn) < LMinQuorumSize(s.constants.config)
+    ==> s.t_replicas[0].v.replica.executor.next_op_to_execute.OutstandingOpUnknown?)
+
+    && (s.t_replicas[0].v.nextActionIndex >= 7 || s.t_replicas[0].v.nextActionIndex == 0
+    ==> Get2bCount(s.t_replicas[0].v.replica, opn) < LMinQuorumSize(s.constants.config)
+    )
+
+    && (Get2bCount(s.t_replicas[0].v.replica, opn) == LMinQuorumSize(s.constants.config)
+    ==> TimeLe(s.t_replicas[0].dts, TimeBound2bDelivery(req_time)))
+
+    && (s.t_replicas[0].v.nextActionIndex == 6
+        && Get2bCount(s.t_replicas[0].v.replica, opn) == LMinQuorumSize(s.constants.config)
+    ==> 
+    s.t_replicas[0].v.replica.executor.next_op_to_execute.OutstandingOpKnown?
+    )
+
+    && (s.t_replicas[0].v.replica.executor.next_op_to_execute.OutstandingOpKnown?
+    ==> Get2bCount(s.t_replicas[0].v.replica, opn) == LMinQuorumSize(s.constants.config)
+    )
+
     && ProposedLeaderNextOperationNumberInvariant(s.t_replicas[0].v.replica.proposer, s.t_replicas[0].v.replica.acceptor.log_truncation_point)
 
-    && (var num_2bs := if opn in s.t_replicas[0].v.replica.learner.unexecuted_learner_state then |s.t_replicas[0].v.replica.learner.unexecuted_learner_state[opn].received_2b_message_senders| else 0;
+    && (var num_2bs := Get2bCount(s.t_replicas[0].v.replica, opn);
      TimeLe(s.t_replicas[0].ts, TimeBoundPhase2Leader(s.t_replicas[0].dts, num_2bs + 2, s.t_replicas[0].v.nextActionIndex))
     )
     && !progresses[s.constants.config.replica_ids[0]].P2a?
-    && (opn in s.t_replicas[0].v.replica.learner.unexecuted_learner_state ==>
-      (forall id :: id in s.t_replicas[0].v.replica.learner.unexecuted_learner_state[opn].received_2b_message_senders ==> progresses[id] == P2done)
+
+    && (forall opn' :: opn' in s.t_replicas[0].v.replica.learner.unexecuted_learner_state ==>
+    opn' == opn
     )
+
+    &&(BalLeq(s.t_replicas[0].v.replica.learner.max_ballot_seen, Ballot(1, 0))
+    )
+
+    && (opn in s.t_replicas[0].v.replica.learner.unexecuted_learner_state ==>
+    && s.t_replicas[0].v.replica.learner.max_ballot_seen == Ballot(1, 0)
+    && (forall id :: id in s.t_replicas[0].v.replica.learner.unexecuted_learner_state[opn].received_2b_message_senders ==> id in s.constants.config.replica_ids)
+      && (forall id :: id in s.t_replicas[0].v.replica.learner.unexecuted_learner_state[opn].received_2b_message_senders ==> progresses[id] == P2done)
+    )
+
   )
 }
 
-predicate {:verify false} Phase2CompletedInvariant(s:TimestampedRslState, req_time:Timestamp, opn:OperationNumber, t2a:Timestamp, progresses:map<NodeIdentity, Phase2Progress>)
+predicate Phase2CompletedInvariant(s:TimestampedRslState, req_time:Timestamp, opn:OperationNumber)
+  requires RslConsistency(s)
 {
-  && GenericPhase2Invariant(s, req_time, t2a, progresses)
+  && PerformanceGuarantee(s, req_time)
+    && (0 < |s.t_replicas|
+    ==>
+    // s.t_replicas[0].v.replica.executor.ops_complete > opn
+    s.t_replicas[0].ts <= TimeBoundPhase2Leader(TimeBound2bDelivery(req_time), LMinQuorumSize(s.constants.config) + 2, 7)
+    )
 }
 
 lemma {:verify false} lemma_leader_3_Pre2aGoesToPhase2UnacceptedLeader(s:TimestampedRslState, s':TimestampedRslState, j:int, req_time:Timestamp, opn:OperationNumber) returns
@@ -340,8 +413,8 @@ lemma {:verify false} lemma_leader_3_Pre2aGoesToPhase2UnacceptedLeader(s:Timesta
     );
   {
     var untagged_pkt := sent_packets[i];
-    var j:int :| 0 <= j < |ios| && ios[j] == LIoOpSend(sent_packets[i]);
-    var pkt := t_ios[j].s;
+    var k:int :| 0 <= k < |ios| && ios[k] == LIoOpSend(sent_packets[i]);
+    var pkt := t_ios[k].s;
 
     progresses' := progresses'[s.constants.config.replica_ids[i] := P2a(pkt)];
     i := i + 1;
@@ -349,7 +422,7 @@ lemma {:verify false} lemma_leader_3_Pre2aGoesToPhase2UnacceptedLeader(s:Timesta
   t2a := s'.t_replicas[0].ts;
 }
 
-lemma {:verify false} lemma_notleader_notreceive_P2UnacceptedGoesToP2Unaccepted(s:TimestampedRslState, s':TimestampedRslState, j:int, req_time:Timestamp, opn:OperationNumber, t2a:Timestamp, progresses:map<NodeIdentity, Phase2Progress>)
+lemma lemma_notleader_notreceive_P2UnacceptedGoesToP2Unaccepted(s:TimestampedRslState, s':TimestampedRslState, j:int, req_time:Timestamp, opn:OperationNumber, t2a:Timestamp, progresses:map<NodeIdentity, Phase2Progress>)
   returns (progresses':map<NodeIdentity,Phase2Progress>)
 
   requires RslAssumption(s);
@@ -374,6 +447,8 @@ lemma {:verify false} lemma_notleader_notreceive_P2UnacceptedGoesToP2Unaccepted(
   progresses' := progresses;
   var t_ios := s.t_environment.nextStep.ios;
   var sent_packets := ExtractSentPacketsFromIos(UntagLIoOpSeq(t_ios));
+  assert ReplicasDistinct(s.constants.config.replica_ids, 0, j);
+
 
   if (LExecutorExecute.requires(s.t_replicas[j].v.replica.executor, s'.t_replicas[j].v.replica.executor, sent_packets)
   && LExecutorExecute(s.t_replicas[j].v.replica.executor, s'.t_replicas[j].v.replica.executor, sent_packets)) {
@@ -386,22 +461,19 @@ lemma {:verify false} lemma_notleader_notreceive_P2UnacceptedGoesToP2Unaccepted(
 
     assert sent_packets == GetPacketsFromReplies(e.constants.all.config.replica_ids[e.constants.my_index], batch, replies);
 
-    forall i |
-      0 <= i < |sent_packets|
-
+    forall i | 0 <= i < |sent_packets|
       ensures sent_packets[i].dst in s.constants.config.clientIds
       ensures sent_packets[i].dst !in s.constants.config.replica_ids
     {
       lemma_SizeOfGetPacketsFromReplies(s.constants.config.replica_ids[j], batch, replies, sent_packets);
       lemma_SpecificPacketInGetPacketsFromReplies(s.constants.config.replica_ids[j], batch, replies, sent_packets, i);
-      assert sent_packets[i].dst == batch[i].client;
-      assert batch[i].client in s.constants.config.clientIds;
+      assert sent_packets[i] == LPacket(batch[i].client, s.constants.config.replica_ids[j], RslMessage_Reply(batch[i].seqno, replies[i].reply));
     }
   } else {
   }
 }
 
-lemma {:verify false} lemma_notleader_receive_P2UnacceptedGoesToP2Unaccepted(s:TimestampedRslState, s':TimestampedRslState, j:int, req_time:Timestamp, opn:OperationNumber, t2a:Timestamp, progresses:map<NodeIdentity, Phase2Progress>)
+lemma lemma_notleader_receive_P2UnacceptedGoesToP2Unaccepted(s:TimestampedRslState, s':TimestampedRslState, j:int, req_time:Timestamp, opn:OperationNumber, t2a:Timestamp, progresses:map<NodeIdentity, Phase2Progress>)
   returns (progresses':map<NodeIdentity,Phase2Progress>)
 
   requires RslAssumption(s);
@@ -465,7 +537,7 @@ lemma {:verify false} lemma_notleader_receive_P2UnacceptedGoesToP2Unaccepted(s:T
   }
 }
 
-lemma {:verify false} lemma_leader_notreceive_P2UnacceptedGoesToP2Unaccepted(s:TimestampedRslState, s':TimestampedRslState, j:int, req_time:Timestamp, opn:OperationNumber, t2a:Timestamp, progresses:map<NodeIdentity, Phase2Progress>)
+lemma lemma_leader_notreceive_P2UnacceptedGoesToP2Unaccepted(s:TimestampedRslState, s':TimestampedRslState, j:int, req_time:Timestamp, opn:OperationNumber, t2a:Timestamp, progresses:map<NodeIdentity, Phase2Progress>)
   returns (progresses':map<NodeIdentity,Phase2Progress>)
 
   requires RslAssumption(s);
@@ -489,7 +561,7 @@ lemma {:verify false} lemma_leader_notreceive_P2UnacceptedGoesToP2Unaccepted(s:T
   progresses' := progresses;
 }
 
-lemma {:verify false} lemma_leader_receive_P2UnacceptedGoesToP2(s:TimestampedRslState, s':TimestampedRslState, j:int, req_time:Timestamp, opn:OperationNumber, t2a:Timestamp, progresses:map<NodeIdentity, Phase2Progress>)
+lemma lemma_leader_receive_P2UnacceptedGoesToP2(s:TimestampedRslState, s':TimestampedRslState, j:int, req_time:Timestamp, opn:OperationNumber, t2a:Timestamp, progresses:map<NodeIdentity, Phase2Progress>)
   returns (progresses':map<NodeIdentity,Phase2Progress>)
 
   requires RslAssumption(s);
@@ -525,19 +597,18 @@ lemma {:verify false} lemma_leader_receive_P2UnacceptedGoesToP2(s:TimestampedRsl
     assert ios[0].r == pkt_2a;
     assert ios[0].r.src == s.constants.config.replica_ids[0];
     BoundedLagImpliesBoundedProcessingTime(s.t_replicas[j].dts, s.t_replicas[j].ts, ios[0].r.msg.ts, s'.t_replicas[j].ts, TimeActionRange(0) + TimeActionRange(0));
-    // t2a + SelfDelivery + 2*TimeActionRange(0) + SelfDelivery
-    // Assume SelfDelivery + TimeActionRange(0) < Delivery
     progresses' := progresses[s.constants.config.replica_ids[0] := P2b];
-    // assert Phase1PreparedLeaderInvariant(s', received_1b_ids, progresses');
+    // assert s.t_replicas[0].ts <= s.t_replicas[0].dts + TimeActionRange(0) + TimeActionRange(s.t_replicas[0].v.nextActionIndex);
+    assert s'.t_replicas[0].ts <= s'.t_replicas[0].dts + TimeActionRange(0) + TimeActionRange(0) + ProcessPacket;
     assert Phase2AcceptedLeaderInvariant(s', req_time, opn, t2a, progresses');
+
   } else {
     progresses' := progresses;
-    // assert Phase1UnpreparedLeaderInvariant(s', pkt, progresses');
     assert Phase2UnacceptedLeaderInvariant(s', req_time, opn, t2a, progresses');
   }
 }
 
-lemma {:verify false} lemma_notleader_notreceive_P2GoesToP2(s:TimestampedRslState, s':TimestampedRslState, j:int, req_time:Timestamp, opn:OperationNumber, t2a:Timestamp, progresses:map<NodeIdentity, Phase2Progress>)
+lemma lemma_notleader_notreceive_P2GoesToP2(s:TimestampedRslState, s':TimestampedRslState, j:int, req_time:Timestamp, opn:OperationNumber, t2a:Timestamp, progresses:map<NodeIdentity, Phase2Progress>)
   returns (progresses':map<NodeIdentity,Phase2Progress>)
 
   requires RslAssumption(s);
@@ -561,6 +632,7 @@ lemma {:verify false} lemma_notleader_notreceive_P2GoesToP2(s:TimestampedRslStat
   progresses' := progresses;
   var t_ios := s.t_environment.nextStep.ios;
   var sent_packets := ExtractSentPacketsFromIos(UntagLIoOpSeq(t_ios));
+  assert ReplicasDistinct(s.constants.config.replica_ids, 0, j);
 
   if (LExecutorExecute.requires(s.t_replicas[j].v.replica.executor, s'.t_replicas[j].v.replica.executor, sent_packets)
   && LExecutorExecute(s.t_replicas[j].v.replica.executor, s'.t_replicas[j].v.replica.executor, sent_packets)) {
@@ -588,7 +660,7 @@ lemma {:verify false} lemma_notleader_notreceive_P2GoesToP2(s:TimestampedRslStat
   }
 }
 
-lemma {:verify false} lemma_notleader_receive_P2GoesToP2(s:TimestampedRslState, s':TimestampedRslState, j:int, req_time:Timestamp, opn:OperationNumber, t2a:Timestamp, progresses:map<NodeIdentity, Phase2Progress>)
+lemma lemma_notleader_receive_P2GoesToP2(s:TimestampedRslState, s':TimestampedRslState, j:int, req_time:Timestamp, opn:OperationNumber, t2a:Timestamp, progresses:map<NodeIdentity, Phase2Progress>)
   returns (progresses':map<NodeIdentity,Phase2Progress>)
 
   requires RslAssumption(s);
@@ -639,7 +711,7 @@ lemma {:verify false} lemma_notleader_receive_P2GoesToP2(s:TimestampedRslState, 
   }
 }
 
-lemma lemma_leader_notreceive_P2GoesToP2(s:TimestampedRslState, s':TimestampedRslState, j:int, req_time:Timestamp, opn:OperationNumber, t2a:Timestamp, progresses:map<NodeIdentity, Phase2Progress>)
+lemma lemma_leader_notreceiveOrExecute_P2GoesToP2(s:TimestampedRslState, s':TimestampedRslState, j:int, req_time:Timestamp, opn:OperationNumber, t2a:Timestamp, progresses:map<NodeIdentity, Phase2Progress>)
   returns (progresses':map<NodeIdentity,Phase2Progress>)
 
   requires RslAssumption(s);
@@ -662,6 +734,85 @@ lemma lemma_leader_notreceive_P2GoesToP2(s:TimestampedRslState, s':TimestampedRs
 {
   reveal_Progress2aProperty();
   progresses' := progresses;
+}
+
+lemma lemma_leader_execute_P2GoesToP2(s:TimestampedRslState, s':TimestampedRslState, j:int, req_time:Timestamp, opn:OperationNumber, t2a:Timestamp, progresses:map<NodeIdentity, Phase2Progress>)
+  returns (progresses':map<NodeIdentity,Phase2Progress>)
+
+  requires RslAssumption(s);
+  requires RslAssumption(s');
+  requires RslConsistency(s);
+  requires RslConsistency(s');
+  requires 0 <= j < |s.constants.config.replica_ids|;
+
+  requires j == 0;
+
+  requires s.t_environment.nextStep.LEnvStepHostIos?;
+  requires s.t_environment.nextStep.actor == s.constants.config.replica_ids[j];
+  requires s.t_environment.nextStep.nodeStep == RslStep(6);
+
+  requires TimestampedRslNextOneReplica(s, s', j, s.t_environment.nextStep.ios);
+
+  requires Phase2AcceptedLeaderInvariant(s, req_time, opn, t2a, progresses)
+  ensures Phase2AcceptedLeaderInvariant(s', req_time, opn, t2a, progresses') || Phase2CompletedInvariant(s', req_time, opn)
+{
+  reveal_Progress2aProperty();
+  progresses' := progresses;
+
+  if (Get2bCount(s.t_replicas[0].v.replica, opn) >= LMinQuorumSize(s.constants.config)) {
+
+    assert Get2bCount(s.t_replicas[0].v.replica, opn) == LMinQuorumSize(s.constants.config);
+    assert TimeLe(s.t_replicas[0].ts, TimeBoundPhase2Leader(s.t_replicas[0].dts, Get2bCount(s.t_replicas[0].v.replica, opn) + 2, s.t_replicas[0].v.nextActionIndex));
+    assert TimeLe(s'.t_replicas[0].ts, TimeBoundPhase2Leader(s'.t_replicas[0].dts, LMinQuorumSize(s.constants.config) + 2, s'.t_replicas[0].v.nextActionIndex));
+    assert Phase2CompletedInvariant(s', req_time, opn);
+  } else {
+    assert Phase2AcceptedLeaderInvariant(s', req_time, opn, t2a, progresses');
+  }
+}
+
+
+lemma lemma_leader_receive_P2GoesToP2(s:TimestampedRslState, s':TimestampedRslState, j:int, req_time:Timestamp, opn:OperationNumber, t2a:Timestamp, progresses:map<NodeIdentity, Phase2Progress>)
+  returns (progresses':map<NodeIdentity,Phase2Progress>)
+
+  requires RslAssumption(s);
+  requires RslAssumption(s');
+  requires RslConsistency(s);
+  requires RslConsistency(s');
+  requires 0 <= j < |s.constants.config.replica_ids|;
+
+  requires j == 0;
+
+  requires s.t_environment.nextStep.LEnvStepHostIos?;
+  requires s.t_environment.nextStep.actor == s.constants.config.replica_ids[j];
+  requires s.t_environment.nextStep.nodeStep == RslStep(0);
+
+  requires TimestampedRslNextOneReplica(s, s', j, s.t_environment.nextStep.ios);
+
+  requires Phase2AcceptedLeaderInvariant(s, req_time, opn, t2a, progresses)
+  ensures Phase2AcceptedLeaderInvariant(s', req_time, opn, t2a, progresses')
+{
+  reveal_Progress2aProperty();
+  progresses' := progresses;
+
+  var ios := s.t_environment.nextStep.ios;
+  if ios[0].LIoOpReceive? {
+    assert ios[0].r.msg.v.RslMessage_2b?;
+    var size := Get2bCount(s.t_replicas[0].v.replica, opn);
+    var size' := Get2bCount(s'.t_replicas[0].v.replica, opn);
+    assert size' == size + 1;
+    
+    BoundedSizeLagImpliesBoundedProcessingTime(s.t_replicas[0].dts,
+      s.t_replicas[0].ts,
+      ios[0].r.msg.ts,
+      s'.t_replicas[0].ts,
+      size + 2
+      );
+    progresses' := progresses[ios[0].r.src := P2done];
+  } else {
+    progresses' := progresses;
+    var size := Get2bCount(s.t_replicas[0].v.replica, opn);
+    LeaderTimeoutPreservesPhase2Invariant(s'.t_replicas[0].dts, size + 2, s'.t_replicas[0].v.nextActionIndex);
+  }
 }
 
 }
